DynamoDbEncryption/dafny/DynamoDbEncryption/Model/AwsCryptographyDbEncryptionSdkDynamoDbTypes.dfy
@@ -46,7 +46,10 @@ module {:extern "software.amazon.cryptography.dbencryptionsdk.dynamodb.internald
     nameonly compoundBeacons: Option<CompoundBeaconList> := Option.None ,
     nameonly virtualFields: Option<VirtualFieldList> := Option.None ,
     nameonly encryptedParts: Option<EncryptedPartsList> := Option.None ,
-    nameonly signedParts: Option<SignedPartsList> := Option.None
+    nameonly signedParts: Option<SignedPartsList> := Option.None ,
+    nameonly maximumNumberOfPartitions: Option<PartitionCount> := Option.None ,
+    nameonly defaultNumberOfPartitions: Option<PartitionCount> := Option.None ,
+    nameonly partitionSelector: Option<IPartitionSelector> := Option.None
   )
   type BeaconVersionList = x: seq<BeaconVersion> | IsValid_BeaconVersionList(x) witness *
   predicate method IsValid_BeaconVersionList(x: seq<BeaconVersion>) {
@@ -281,6 +284,14 @@ module {:extern "software.amazon.cryptography.dbencryptionsdk.dynamodb.internald
   datatype GetEncryptedDataKeyDescriptionUnion =
     | header(header: seq<uint8>)
     | item(item: ComAmazonawsDynamodbTypes.AttributeMap)
+  datatype GetPartitionNumberInput = | GetPartitionNumberInput (
+    nameonly item: ComAmazonawsDynamodbTypes.AttributeMap ,
+    nameonly numberOfPartitions: PartitionCount ,
+    nameonly logicalTableName: string
+  )
+  datatype GetPartitionNumberOutput = | GetPartitionNumberOutput (
+    nameonly partitionNumber: PartitionNumber
+  )
   datatype GetPrefix = | GetPrefix (
     nameonly length: int32
   )
@@ -357,6 +368,79 @@ module {:extern "software.amazon.cryptography.dbencryptionsdk.dynamodb.internald
     nameonly cache: Option<AwsCryptographyMaterialProvidersTypes.CacheType> := Option.None ,
     nameonly partitionId: Option<string> := Option.None
   )
+  type PartitionCount = x: int32 | IsValid_PartitionCount(x) witness *
+  predicate method IsValid_PartitionCount(x: int32) {
+    ( 1 <= x <= 255 )
+  }
+  type PartitionNumber = x: int32 | IsValid_PartitionNumber(x) witness *
+  predicate method IsValid_PartitionNumber(x: int32) {
+    ( 0 <= x <= 254 )
+  }
+  class IPartitionSelectorCallHistory {
+    ghost constructor() {
+      GetPartitionNumber := [];
+    }
+    ghost var GetPartitionNumber: seq<DafnyCallEvent<GetPartitionNumberInput, Result<GetPartitionNumberOutput, Error>>>
+  }
+  trait {:termination false} IPartitionSelector
+  {
+    // Helper to define any additional modifies/reads clauses.
+    // If your operations need to mutate state,
+    // add it in your constructor function:
+    // Modifies := {your, fields, here, History};
+    // If you do not need to mutate anything:
+    // Modifies := {History};
+
+    ghost const Modifies: set<object>
+    // For an unassigned field defined in a trait,
+    // Dafny can only assign a value in the constructor.
+    // This means that for Dafny to reason about this value,
+    // it needs some way to know (an invariant),
+    // about the state of the object.
+    // This builds on the Valid/Repr paradigm
+    // To make this kind requires safe to add
+    // to methods called from unverified code,
+    // the predicate MUST NOT take any arguments.
+    // This means that the correctness of this requires
+    // MUST only be evaluated by the class itself.
+    // If you require any additional mutation,
+    // then you MUST ensure everything you need in ValidState.
+    // You MUST also ensure ValidState in your constructor.
+    predicate ValidState()
+      ensures ValidState() ==> History in Modifies
+    ghost const History: IPartitionSelectorCallHistory
+    predicate GetPartitionNumberEnsuresPublicly(input: GetPartitionNumberInput , output: Result<GetPartitionNumberOutput, Error>)
+    // The public method to be called by library consumers
+    method GetPartitionNumber ( input: GetPartitionNumberInput )
+      returns (output: Result<GetPartitionNumberOutput, Error>)
+      requires
+        && ValidState()
+      modifies Modifies - {History} ,
+               History`GetPartitionNumber
+      // Dafny will skip type parameters when generating a default decreases clause.
+      decreases Modifies - {History}
+      ensures
+        && ValidState()
+      ensures GetPartitionNumberEnsuresPublicly(input, output)
+      ensures History.GetPartitionNumber == old(History.GetPartitionNumber) + [DafnyCallEvent(input, output)]
+    {
+      output := GetPartitionNumber' (input);
+      History.GetPartitionNumber := History.GetPartitionNumber + [DafnyCallEvent(input, output)];
+    }
+    // The method to implement in the concrete class.
+    method GetPartitionNumber' ( input: GetPartitionNumberInput )
+      returns (output: Result<GetPartitionNumberOutput, Error>)
+      requires
+        && ValidState()
+      modifies Modifies - {History}
+      // Dafny will skip type parameters when generating a default decreases clause.
+      decreases Modifies - {History}
+      ensures
+        && ValidState()
+      ensures GetPartitionNumberEnsuresPublicly(input, output)
+      ensures unchanged(History)
+
+  }
   datatype PartOnly = | PartOnly (
 
                       )
@@ -397,7 +481,8 @@ module {:extern "software.amazon.cryptography.dbencryptionsdk.dynamodb.internald
     nameonly name: string ,
     nameonly length: BeaconBitLength ,
     nameonly loc: Option<TerminalLocation> := Option.None ,
-    nameonly style: Option<BeaconStyle> := Option.None
+    nameonly style: Option<BeaconStyle> := Option.None ,
+    nameonly numberOfPartitions: Option<PartitionCount> := Option.None
   )
   type StandardBeaconList = x: seq<StandardBeacon> | IsValid_StandardBeaconList(x) witness *
   predicate method IsValid_StandardBeaconList(x: seq<StandardBeacon>) {
